\subsection{Strong Mathematical Induction}
\hrulefill

\subsubsection*{Principle of Strong Mathematical Induction}
Let P(n) be a property that is defined for integers n, and let a and b be fixed integers with $a \leq b$.
\begin{itemize}
    \item Basis Step: Show that P(a), P(a+1), \dots, P(b) are all true.
    \item Inductive Step: Show that for every ingeger $k \geq b$, if P(a), P(a+1), \dots, P(k) are all true, then P(k+1) is true.
\end{itemize}

\paragraph*{Example}
Define a sequence:
\begin{align*}
    S_0 &= 0\\
    S_1 &= 4\\
    \forall k \in \{x \in \mathbb{Z} : x \geq 2\}, S_k &= 6S_{k-1} - 5S_{k-2}\\
\end{align*}
Prove $\forall n \in \{x \in \mathbb{Z} : x \geq 0\}, S_n = 5^n - 1$:
\begin{align*}
    &\text{Let } G = \{x \in \mathbb{Z} : x \geq 0\}\\
    \\
    &\text{Basic step:}\\
    &\quad S_0 = 5^0 - 1 = 1 - 1 = 0\\
    &\quad S_1 = 5^1 - 1 = 5 - 1 = 4\\
    \\
    &\text{Inductive step:}\\
    &\quad \text{Suppose } \forall k \in G, S_k = 5^k - 1\\
    \implies& \quad S_{k+1} = 6S_k - 5S_{k-1} = 6(5^k-1) - 5(5^{k-1}-1) = 6(5^k) - 6 + 5(5^{k-1}) + 5\\
    &\quad = 6(5^k) - (5^{k-1+1}) - 1 = (6-1)5^k - 1 = 5 \cdot 5^k - 1 = 5^{k+1} - 1\\
    &\therefore \quad S_{k+1} = 6S_k - 5S_{k-1}\\
    \therefore &\quad \forall n \in \{x \in \mathbb{Z} : x \geq 0\}, S_n = 5^n - 1
\end{align*}

