\subsection{Solving Recurrence relations by Iteration}
\hrulefill\\
\paragraph*{Method}
Starting from the initial conditions, calculate the successive terms of sequences from the recurrence formula until a pattern emerges. 
Then, use the pattern to find a closed form for the sequence.

\paragraph*{Example}
\begin{equation*}
    a_n =
    \begin{cases}
        1, & n = 0\\
        a_{n-1} + 2, & \forall n \in \mathbb{Z}^+\\
    \end{cases}
\end{equation*}
Solve the recurrence relation.
\begin{align*}
    \forall n \in \mathbb{Z}^+, a_k = a_{k-1} + 2\\
    a_n = (a_{n-1} + 2) + 2\\
    a_n = (a_{n-2} + 2) + 2(2)\\
    \cdots\\
    a_n = a_{n-k} + k(2)\\
    \therefore \quad \forall n \in \mathbb{Z}^+, \quad a_n = a_0 + 2n\\
    \therefore \quad \forall n \in \mathbb{Z}^+, \quad a_n = 1 + 2n
\end{align*}

\subsubsection*{Arithmetic Sequence}
\paragraph*{Definition}
A sequence is arithmetic if there is a constant $d$ such that:
\begin{equation*}
    \forall k \in \mathbb{Z}^+, \quad  a_k = a_{k-1} + d
\end{equation*}
\paragraph*{General Formula}
\begin{equation*}
    \forall n \in \{x \in \mathbb{Z} : x \geq 0}, \quad a_n = a_0 + nd
\end{equation*}

\subsubsection*{Geometric Sequence}
\paragraph*{Definition}
A sequence is geometric if there is a constant $r$ such that:
\begin{equation*}
    \forall k \in \mathbb{Z}^+, \quad  a_k = a_{k-1}r
\end{equation*}
\paragraph*{General Formula}
\begin{equation*}
    \forall n \in \{x \in \mathbb{Z} : x \geq 0\}, \quad a_n = a_0 r^n
\end{equation*}

\paragraph*{Example}
Use iteration to find the explicit formula of the following sequence:
\begin{equation*}
    e_k = 
    \begin{cases}
        2, & k = 0\\
        4e_{k-1} + 5, & k \geq 0
    \end{cases}
\end{equation*}

\begin{align*}
    e_0 &= 2\\
    e_1 &= 4(2) + 5\\
    e_2 &= 4(4(2) + 5) + 5 = 4^2(2) + 4(5) + 5\\
    e_3 &= 4(4^2(2) + 4(5) + 5) + 5 = 4^3(2) + 4^2(5) + 4(5) + 5\\
    &\cdots\\
    e_k &= 4^k(2) + 4^{k-1}(5) + 4^{k-2}(5) + \cdots + 4(5) + 5\\
    &= 4^k(2) + 5 \sum_{i=0}^{k-1} 4^i = 4^k(2) + 5 (\frac{4^{k-1+1} - 1}{4 - 1})\\
    e_k &= 4^k(2) + 5 (\frac{4^{k} - 1}{3})\\
\end{align*}

